done

dev2016/fsub.v
@@ -227,7 +227,7 @@ Inductive stp2: bool (* whether the last rule may not be transitivity *) ->
 | stp2_sel1: forall G1 G2 GX TX x T2 GH n1,
     indexr x G1 = Some (vty GX TX) ->
     closed 0 0 (length GX) TX ->
-    stp2 false GX TX G2 T2 GH n1 ->
+    stp2 true GX TX G2 T2 GH n1 ->
     stp2 true G1 (TVarF x) G2 T2 GH (S n1)
 | stp2_sel2: forall G1 G2 GX TX x T1 GH n1,
     indexr x G2 = Some (vty GX TX) ->
@@ -1562,7 +1562,7 @@ Proof. intros. repeat eu. eauto. Qed.
 Lemma stpd2_sel1: forall G1 G2 GX TX x T2 GH,
     indexr x G1 = Some (vty GX TX) ->
     closed 0 0 (length GX) TX ->
-    stpd2 false GX TX G2 T2 GH ->
+    stpd2 true GX TX G2 T2 GH ->
     stpd2 true G1 (TVarF x) G2 T2 GH.
 Proof. intros. repeat eu. eauto. Qed.
 Lemma stpd2_sel2: forall G1 G2 GX TX x T1 GH,
@@ -1728,15 +1728,16 @@ Ltac indexr_contra :=
     | H: indexr ?N [] = Some ?V |- _ => simpl in H; inversion H
   end.
 
-Lemma stpd2_untrans_aux: forall n, forall m G1 G2 G3 T1 T2 T3 n1,
-  stp2 m G1 T1 G2 T2 nil n1 -> n1 < n ->
-  stpd2 true G2 T2 G3 T3 nil ->
-  stpd2 true G1 T1 G3 T3 nil.
+Lemma stpd2_untrans_aux: forall n, forall m G1 G2 G3 T1 T2 T3 GH n1,
+  stp2 m G1 T1 G2 T2 GH n1 -> n1 < n ->
+  stpd2 true G2 T2 G3 T3 GH ->
+  stpd2 true G1 T1 G3 T3 GH.
 Proof.
   intros n. induction n; intros; try omega. eu.
   inversion H; subst;
   try solve [inversion H1; eexists; eauto];
-  try solve [eapply stpd2_sel1; eauto; eapply stpd2_wrapf; eapply IHn; eauto; try omega];
+  try solve [eapply stpd2_sel1; eauto; eapply IHn; eauto; try omega];
+  try solve [eapply stpd2_sela1; eauto; eapply stpd2_wrapf; eapply IHn; eauto; try omega];
   try solve [eapply IHn; [eapply H2 | omega | eauto]]; (* wrapf *)
   try solve [eapply IHn; [eapply H2 | omega | (eapply IHn; [ eapply H3 | omega | eauto ])]]; (* transf *)
   inversion H1; subst;
@@ -1748,8 +1749,7 @@ Proof.
   try solve [indexr_contra].
   - Case "sel2 - sel1".
     rewrite H6 in H2. inversion H2. subst.
-    eapply IHn. eapply H4. omega.
-    admit.
+    eapply IHn. eapply H4. omega. eauto.
   - Case "sel2 - selx".
     rewrite H6 in H2. inversion H2. subst.
     eapply stpd2_sel2; eauto.
@@ -1759,6 +1759,8 @@ Proof.
   - Case "selx - selx".
     rewrite H5 in H3. inversion H3. subst.
     eapply stpd2_selx; eauto.
+  - Case "selax - selax".
+    eapply stpd2_selax; eauto.
   - Case "all - all".
     eapply stpd2_all; eauto.
     eapply stpd2_trans; eauto.
@@ -1766,15 +1768,15 @@ Proof.
 Grab Existential Variables. apply 0.
 Qed.
 
-Lemma stpd2_untrans: forall G1 G2 G3 T1 T2 T3,
-  stpd2 true G1 T1 G2 T2 nil ->
-  stpd2 true G2 T2 G3 T3 nil ->
-  stpd2 true G1 T1 G3 T3 nil.
+Lemma stpd2_untrans: forall G1 G2 G3 T1 T2 T3 GH,
+  stpd2 true G1 T1 G2 T2 GH ->
+  stpd2 true G2 T2 G3 T3 GH ->
+  stpd2 true G1 T1 G3 T3 GH.
 Proof. intros. repeat eu. eapply stpd2_untrans_aux; eauto. Qed.
 
-Lemma stpd2_upgrade: forall G1 G2 T1 T2,
-  stpd2 false G1 T1 G2 T2 [] ->
-  stpd2 true G1 T1 G2 T2 [].
+Lemma stpd2_upgrade: forall G1 G2 T1 T2 GH,
+  stpd2 false G1 T1 G2 T2 GH ->
+  stpd2 true G1 T1 G2 T2 GH.
 Proof.
   intros. destruct H as [n H].
   eapply stpd2_untrans_aux; eauto using stp2_reg2.
@@ -2285,14 +2287,14 @@ Lemma stp2_substitute_aux: forall n, forall G1 G2 T1 T2 GH m n1,
      compat GX TX G1 T1 T1' ->
      compat GX TX G2 T2 T2' ->
      Forall2 (compat2 GX TX) GH0 GH0' ->
-     stpd2 false G1 T1' G2 T2' GH0'.
+     stpd2 m G1 T1' G2 T2' GH0'.
 Proof.
   intros n. induction n.
   Case "z". intros. inversion H0. subst. inversion H; eauto.
   intros G1 G2 T1 T2 GH m n1 H NE.
   induction H.
   - Case "top".
-    intros GH0 GH0' GXX TXX T1' T2' ? CX IX1 IX2 FA; eapply stpd2_wrapf.
+    intros GH0 GH0' GXX TXX T1' T2' ? CX IX1 IX2 FA.
     eapply compat_top in IX2.
     subst. eapply stpd2_top.
     eapply compat_closed. eassumption.
@@ -2301,7 +2303,7 @@ Proof.
     eassumption. assumption.
 
   - Case "fun".
-    intros GH0 GH0' GXX TXX T1' T2' ? CX IX1 IX2 FA; eapply stpd2_wrapf.
+    intros GH0 GH0' GXX TXX T1' T2' ? CX IX1 IX2 FA.
     eapply compat_fun in IX1. repeat destruct IX1 as [? IX1].
     eapply compat_fun in IX2. repeat destruct IX2 as [? IX2].
     subst. eapply stpd2_fun.
@@ -2309,7 +2311,7 @@ Proof.
     eauto. eauto.
 
   - Case "mem".
-    intros GH0 GH0' GXX TXX T1' T2' ? CX IX1 IX2 FA; eapply stpd2_wrapf.
+    intros GH0 GH0' GXX TXX T1' T2' ? CX IX1 IX2 FA.
     eapply compat_mem in IX1. repeat destruct IX1 as [? IX1].
     eapply compat_mem in IX2. repeat destruct IX2 as [? IX2].
     subst. eapply stpd2_mem.
@@ -2317,7 +2319,7 @@ Proof.
     eauto. eauto.
 
   - Case "sel1".
-    intros GH0 GH0' GXX TXX T1' T2' ? CX IX1 IX2 FA; eapply stpd2_wrapf.
+    intros GH0 GH0' GXX TXX T1' T2' ? CX IX1 IX2 FA.
 
     assert (length GH = length GH0 + 1). subst GH. eapply app_length.
     assert (length GH0 = length GH0') as EL. eapply Forall2_length. eauto.
@@ -2332,7 +2334,7 @@ Proof.
     eauto. eauto. eauto.
 
   - Case "sel2".
-    intros GH0 GH0' GXX TXX T1' T2' ? CX IX1 IX2 FA; eapply stpd2_wrapf.
+    intros GH0 GH0' GXX TXX T1' T2' ? CX IX1 IX2 FA.
 
     assert (length GH = length GH0 + 1). subst GH. eapply app_length.
     assert (length GH0 = length GH0') as EL. eapply Forall2_length. eauto.
@@ -2347,7 +2349,7 @@ Proof.
     eauto. eauto. eauto.
 
   - Case "selx".
-    intros GH0 GH0' GXX TXX T1' T2' ? CX IX1 IX2 FA; eapply stpd2_wrapf.
+    intros GH0 GH0' GXX TXX T1' T2' ? CX IX1 IX2 FA.
 
     assert (length GH = length GH0 + 1). subst GH. eapply app_length.
     assert (length GH0 = length GH0') as EL. eapply Forall2_length. eauto.
@@ -2381,15 +2383,15 @@ Proof.
     + SCase "x = 0".
       repeat destruct IXX as [|IXX]; ev.
       * subst. simpl.
-        eapply stpd2_wrapf. eapply stpd2_sel1. eauto. eauto.
-        eapply IHn; eauto; try omega. right. right. left. auto.
+        eapply stpd2_sel1. eauto. eauto.
+        eapply stpd2_upgrade. eapply IHn; eauto; try omega. right. right. left. auto.
       * subst. simpl.
-        eapply IHstp2; eauto; try omega. right. right. left. auto.
+        eapply stpd2_upgrade. eapply IHn; eauto; try omega. right. right. left. auto.
       * subst. inversion H5. subst. omega.
       * subst. destruct H5. eauto.
     + SCase "x > 0".
       ev. subst.
-      eapply stpd2_wrapf. eapply stpd2_sela1. eauto.
+      eapply stpd2_sela1. eauto.
 
       assert (x-1+1=x) as A by omega.
       remember (x-1) as x1. rewrite <- A in H0.
@@ -2399,7 +2401,7 @@ Proof.
     + eauto. + subst GH. eauto. + eauto.
 
   - Case "selax".
-    intros GH0 GH0' GXX TXX T1' T2' ? CX IX1 IX2 FA; eapply stpd2_wrapf.
+    intros GH0 GH0' GXX TXX T1' T2' ? CX IX1 IX2 FA.
 
     assert (length GH = length GH0 + 1). subst GH. eapply app_length.
     assert (length GH0 = length GH0') as EL. eapply Forall2_length. eauto.
@@ -2419,14 +2421,13 @@ Proof.
       destruct H0. destruct H0. subst. simpl.
       destruct H3. destruct H3. subst. simpl.
       eapply stpd2_sel1. eauto. eauto.
-      eapply stpd2_wrapf. eapply stpd2_sel2. eauto. eauto.
+      eapply stpd2_sel2. eauto. eauto.
       eapply stpd2_wrapf.
       eapply stp2_refl. eapply closed_upgrade_free. eassumption. omega.
 
       destruct H0. destruct H0. subst. simpl.
       destruct H3. destruct H3. subst. simpl.
       eapply stpd2_sel1. eauto. eauto.
-      eapply stpd2_wrapf.
       eapply stp2_refl. eapply closed_upgrade_free. eassumption. omega.
 
       destruct H3. destruct H3. subst. simpl.
@@ -2471,7 +2472,7 @@ Proof.
     + eauto.
 
   - Case "all".
-    intros GH0 GH0' GX TX T1' T2' ? CX IX1 IX2 FA; eapply stpd2_wrapf.
+    intros GH0 GH0' GX TX T1' T2' ? CX IX1 IX2 FA.
 
     assert (length GH = length GH0 + 1). subst GH. eapply app_length.
     assert (length GH0 = length GH0') as EL. eapply Forall2_length. eauto.
@@ -2499,12 +2500,12 @@ Proof.
     + eauto.
     + eauto. subst GH. rewrite <-EL. eapply closed_upgrade_free. eauto. omega.
   - Case "wrapf".
-    intros. subst. eapply IHn; eauto; try omega.
+    intros. subst. eapply stpd2_wrapf; eapply IHn; eauto; try omega.
   - Case "transf".
     intros. subst.
     apply stp2_extend2 with (v1:=(vty GX TX)) in H.
     apply stp2_extend1 with (v1:=(vty GX TX)) in H0.
-    eapply stpd2_trans.
+    eapply stpd2_transf.
 
     eapply IHn; eauto; try omega.
     unfold compat. simpl. left. exists (length G2).
@@ -2523,7 +2524,7 @@ Lemma stp2_substitute: forall G1 G2 T1 T2 GH m,
      compat GX TX G1 T1 T1' ->
      compat GX TX G2 T2 T2' ->
      Forall2 (compat2 GX TX) GH0 GH0' ->
-     stpd2 false G1 T1' G2 T2' GH0'.
+     stpd2 m G1 T1' G2 T2' GH0'.
 Proof.
   intros. repeat eu. eapply stp2_substitute_aux; eauto.
 Qed.
@@ -2549,6 +2550,7 @@ Proof.
     eapply stpd2_sel1; eauto. inversion H2. subst.
     eapply stp2_closed1 in H3. eauto. inversion H3. subst. simpl in H9. apply H9.
     eapply stp2_closed1 in H3. eauto. inversion H3. subst. simpl in H13. apply H13.
+    eapply stpd2_upgrade.
     eapply stpd2_trans. eexists. apply H7. eapply IHST; eauto.
     destruct H5 as [? H5]. inversion H5.
     destruct H5 as [? H5]. inversion H5.
